Commit WIP stuff

Graphiti/Core/Environment.lean
@@ -16,21 +16,28 @@ namespace Graphiti
 
 def Env Ident Typ := Typ → Option (TModule1 Ident)
 
+abbrev FinEnv Ident Typ := Batteries.AssocList Typ (TModule1 Ident)
+
 namespace Env
 
 def subsetOf {Ident Typ} (ε₁ ε₂ : Env Ident Typ) : Prop :=
   ∀ i v, ε₁ i = .some v → ε₂ i = .some v
 
-def well_formed (ε : Env String (String × String)) (s : String) : Prop :=
+def union {Ident Typ} (ε₁ ε₂ : Env Ident Typ) : Env Ident Typ := λ s =>
+  match ε₁ s with
+  | some x => pure x
+  | none => ε₂ s
+
+def well_formed {α} (ε : Env String (String × α)) (s : String) : Prop :=
   match s with
   | "branch" => ∀ a mod, ε (s, a) = some mod → ∃ T, mod = ⟨_, StringModule.branch T⟩
   | "cntrl_merge" => ∀ a mod, ε (s, a) = some mod → ∃ T, mod = ⟨_, StringModule.cntrl_merge T⟩
   | "constant" => ∀ a mod, ε (s, a) = some mod → ∃ T, ∃ (t : T), mod = ⟨_, StringModule.constant t⟩
-  | "fork" => ∀ a mod, ε (s, a) = some mod → ∃ T n, mod = ⟨_, StringModule.fork T n⟩
-  | "init" => ∀ a mod, ε (s, a) = some mod → ∃ T, ∃ (t : T), mod = ⟨_, StringModule.init T t⟩
-  | "join" => ∀ a mod, ε (s, a) = some mod → ∃ T T', mod = ⟨_, StringModule.join T T'⟩
-  | "load" => ∀ a mod, ε (s, a) = some mod → ∃ S T, mod = ⟨_, StringModule.load S T⟩
-  | "merge" => ∀ a mod, ε (s, a) = some mod → ∃ T n, mod = ⟨_, StringModule.merge T n⟩
+  | "fork" => ∀ a mod, ε (s, a) = some mod → ∃ (T : Type _ × Nat), mod = ⟨_, StringModule.fork T.1 T.2⟩
+  | "init" => ∀ a mod, ε (s, a) = some mod → ∃ (T : Sigma id), mod = ⟨_, StringModule.init T.1 T.2⟩
+  | "join" => ∀ a mod, ε (s, a) = some mod → ∃ (T : Type _ × Type _), mod = ⟨_, StringModule.join T.1 T.2⟩
+  | "load" => ∀ a mod, ε (s, a) = some mod → ∃ (T : Type _ × Type _), mod = ⟨_, StringModule.load T.1 T.2⟩
+  | "merge" => ∀ a mod, ε (s, a) = some mod → ∃ (T : Type _ × Nat), mod = ⟨_, StringModule.merge T.1 T.2⟩
   | "mux" => ∀ a mod, ε (s, a) = some mod → ∃ T, mod = ⟨_, StringModule.mux T⟩
   | "operator1" => ∀ a mod, ε (s, a) = some mod → ∃ T1 T2 T2m s, mod = ⟨_, @StringModule.operator1 T1 T2 T2m s⟩
   | "operator2" => ∀ a mod, ε (s, a) = some mod → ∃ T1 T2 T3 T3m s, mod = ⟨_, @StringModule.operator2 T1 T2 T3 T3m s⟩
@@ -43,5 +50,29 @@ def well_formed (ε : Env String (String × String)) (s : String) : Prop :=
   | _ => True
 
 end Env
+
+namespace FinEnv
+
+theorem exists_fresh {Ident} {ε : FinEnv Ident (String × String)} {a : List String}
+  : ∃ (b : List String), a.length = b.length ∧ (∀ a' b', (a', b') ∈ a.zip b → ¬ ε.contains (a', b')) ∧ (a.zip b).Nodup := by sorry
+
+noncomputable def select_fresh' {Ident} (ε : FinEnv Ident (String × String)) (a : List String) : List String :=
+  Exists.choose (@exists_fresh Ident ε a)
+
+theorem select_fresh'_spec {Ident} {ε : FinEnv Ident (String × String)} {a : List String} :
+  a.length = (select_fresh' ε a).length ∧ (∀ a' b', (a', b') ∈ a.zip (select_fresh' ε a) → ¬ ε.contains (a', b')) ∧ (a.zip (select_fresh' ε a)).Nodup :=
+  Exists.choose_spec exists_fresh
+
+noncomputable def select_fresh {Ident} (ε : FinEnv Ident (String × String)) (a : List String) : List (String × String) :=
+  a.zip (select_fresh' ε a)
+
+theorem select_fresh_spec {Ident} {ε : FinEnv Ident (String × String)} {a : List String} :
+  a.length = (select_fresh ε a).length ∧ (∀ a' b', (a', b') ∈ select_fresh ε a → ¬ ε.contains (a', b')) ∧ (select_fresh ε a).Nodup := by
+  grind [select_fresh, select_fresh'_spec]
+
+def max_type {Ident} (f : FinEnv Ident (String × Nat)) : Nat :=
+  f.keysList.map Prod.snd |>.foldl Nat.max 0
+
+end FinEnv
 
 end Graphiti
